Kami/Ex/ProcFCorrect.v
@@ -1,0 +1,66 @@
+Require Import Bool String List.
+Require Import Lib.CommonTactics Lib.ilist Lib.Word.
+Require Import Lib.Struct Lib.FMap Lib.StringEq Lib.Indexer.
+Require Import Kami.Syntax Kami.Semantics Kami.RefinementFacts Kami.Renaming Kami.Wf.
+Require Import Kami.Renaming Kami.Inline Kami.InlineFacts.
+Require Import Kami.Decomposition Kami.Notations Kami.Tactics.
+Require Import Ex.MemTypes Ex.NativeFifo Ex.MemAsync.
+Require Import Ex.SC Ex.ProcDec Ex.ProcThreeStage Ex.ProcFetch Ex.ProcFInl
+        Ex.ProcFetchDecode.
+Require Import Eqdep.
+
+Set Implicit Arguments.
+
+Section Fetch.
+  Variables addrSize iaddrSize instBytes dataBytes: nat.
+
+  Variables (fetch: AbsFetch instBytes dataBytes)
+            (predictNextPc:
+               forall ty, fullType ty (SyntaxKind (Pc iaddrSize)) -> (* pc *)
+                          Expr ty (SyntaxKind (Pc iaddrSize))).
+
+  Variable (f2dElt: Kind).
+  Variable (f2dPack:
+              forall ty,
+                Expr ty (SyntaxKind (Data instBytes)) -> (* rawInst *)
+                Expr ty (SyntaxKind (Pc iaddrSize)) -> (* curPc *)
+                Expr ty (SyntaxKind (Pc iaddrSize)) -> (* nextPc *)
+                Expr ty (SyntaxKind Bool) -> (* epoch *)
+                Expr ty (SyntaxKind f2dElt)).
+  Variables
+    (f2dRawInst: forall ty, fullType ty (SyntaxKind f2dElt) ->
+                            Expr ty (SyntaxKind (Data instBytes)))
+    (f2dCurPc: forall ty, fullType ty (SyntaxKind f2dElt) ->
+                          Expr ty (SyntaxKind (Pc iaddrSize)))
+    (f2dNextPc: forall ty, fullType ty (SyntaxKind f2dElt) ->
+                           Expr ty (SyntaxKind (Pc iaddrSize)))
+    (f2dEpoch: forall ty, fullType ty (SyntaxKind f2dElt) ->
+                          Expr ty (SyntaxKind Bool)).
+
+  Hypotheses (Hf2dRawInst: forall rawInst curPc nextPc epoch,
+                 evalExpr (f2dRawInst _ (evalExpr (f2dPack rawInst curPc nextPc epoch))) =
+                 evalExpr rawInst)
+             (Hf2dCurPc: forall rawInst curPc nextPc epoch,
+                 evalExpr (f2dCurPc _ (evalExpr (f2dPack rawInst curPc nextPc epoch))) =
+                 evalExpr curPc)
+             (Hf2dNextPc: forall rawInst curPc nextPc epoch,
+                 evalExpr (f2dNextPc _ (evalExpr (f2dPack rawInst curPc nextPc epoch))) =
+                 evalExpr nextPc)
+             (Hf2dEpoch: forall rawInst curPc nextPc epoch,
+                 evalExpr (f2dEpoch _ (evalExpr (f2dPack rawInst curPc nextPc epoch))) =
+                 evalExpr epoch).
+
+  Variables (pcInit : ConstT (Pc iaddrSize)).
+
+  Definition fetchICache: Modules :=
+    fetchICache addrSize fetch predictNextPc f2dPack pcInit.
+  Definition fetcher: Modules :=
+    ProcFetchDecode.fetcher addrSize fetch predictNextPc f2dPack pcInit.
+
+  Theorem fetchICache_refines_fetcher:
+    fetchICache <<== fetcher.
+  Proof.
+  Admitted.
+
+End Fetch.
+
