Kami/Ex/ProcFInl.v
@@ -1,0 +1,45 @@
+Require Import Bool String List.
+Require Import Kami.Syntax Kami.Semantics Kami.RefinementFacts Kami.Renaming Kami.Wf.
+Require Import Kami.Inline Kami.InlineFacts Kami.Tactics.
+Require Import Ex.SC Ex.MemTypes Ex.ProcFetch.
+
+Set Implicit Arguments.
+
+Section Inlined.
+  Variables addrSize iaddrSize instBytes dataBytes rfIdx: nat.
+
+  Variables (fetch: AbsFetch instBytes dataBytes)
+            (predictNextPc:
+               forall ty, fullType ty (SyntaxKind (Pc iaddrSize)) -> (* pc *)
+                          Expr ty (SyntaxKind (Pc iaddrSize))).
+
+  Variable (f2dElt: Kind).
+  Variable (f2dPack:
+              forall ty,
+                Expr ty (SyntaxKind (Data instBytes)) -> (* rawInst *)
+                Expr ty (SyntaxKind (Pc iaddrSize)) -> (* curPc *)
+                Expr ty (SyntaxKind (Pc iaddrSize)) -> (* nextPc *)
+                Expr ty (SyntaxKind Bool) -> (* epoch *)
+                Expr ty (SyntaxKind f2dElt)).
+  Variables
+    (f2dRawInst: forall ty, fullType ty (SyntaxKind f2dElt) ->
+                            Expr ty (SyntaxKind (Data instBytes)))
+    (f2dCurPc: forall ty, fullType ty (SyntaxKind f2dElt) ->
+                          Expr ty (SyntaxKind (Pc iaddrSize)))
+    (f2dNextPc: forall ty, fullType ty (SyntaxKind f2dElt) ->
+                           Expr ty (SyntaxKind (Pc iaddrSize)))
+    (f2dEpoch: forall ty, fullType ty (SyntaxKind f2dElt) ->
+                          Expr ty (SyntaxKind Bool)).
+
+  Variables (pcInit : ConstT (Pc iaddrSize)).
+
+  Definition fetchICache :=
+    fetchICache addrSize fetch predictNextPc f2dPack pcInit.
+  Hint Unfold fetchICache: ModuleDefs. (* for kinline_compute *)
+
+  Definition fetchICacheInl: sigT (fun m: Modules => fetchICache <<== m).
+  Proof.
+    kinline_refine fetchICache.
+  Defined.
+
+End Inlined.
