Kami/Ex/ProcFetch.v
@@ -1,0 +1,230 @@
+Require Import Bool String List.
+Require Import Lib.CommonTactics Lib.ilist Lib.Word Lib.Indexer.
+Require Import Kami.Syntax Kami.Notations Kami.Semantics Kami.Specialize Kami.Duplicate.
+Require Import Kami.Wf Kami.Tactics.
+Require Import Ex.MemTypes Ex.SC Ex.OneEltFifo Ex.Fifo Ex.MemAsync Ex.ProcFetchDecode.
+Require Import Kami.PrimBram.
+
+Set Implicit Arguments.
+
+Section FetchICache.
+  Variables addrSize iaddrSize instBytes dataBytes rfIdx: nat.
+
+  Variables (fetch: AbsFetch instBytes dataBytes)
+            (predictNextPc:
+               forall ty, fullType ty (SyntaxKind (Pc iaddrSize)) -> (* pc *)
+                          Expr ty (SyntaxKind (Pc iaddrSize))).
+
+  Variable (f2dElt: Kind).
+  Variable (f2dPack:
+              forall ty,
+                Expr ty (SyntaxKind (Data instBytes)) -> (* rawInst *)
+                Expr ty (SyntaxKind (Pc iaddrSize)) -> (* curPc *)
+                Expr ty (SyntaxKind (Pc iaddrSize)) -> (* nextPc *)
+                Expr ty (SyntaxKind Bool) -> (* epoch *)
+                Expr ty (SyntaxKind f2dElt)).
+  Variables
+    (f2dRawInst: forall ty, fullType ty (SyntaxKind f2dElt) ->
+                            Expr ty (SyntaxKind (Data instBytes)))
+    (f2dCurPc: forall ty, fullType ty (SyntaxKind f2dElt) ->
+                          Expr ty (SyntaxKind (Pc iaddrSize)))
+    (f2dNextPc: forall ty, fullType ty (SyntaxKind f2dElt) ->
+                           Expr ty (SyntaxKind (Pc iaddrSize)))
+    (f2dEpoch: forall ty, fullType ty (SyntaxKind f2dElt) ->
+                          Expr ty (SyntaxKind Bool)).
+
+  Definition icache: Modules :=
+    bram1 "pgm" 1 iaddrSize (Data instBytes).
+
+  Definition instRq :=
+    MethodSig ("pgm" -- "putRq")
+              (Struct (BramRq iaddrSize (Data instBytes))): Void.
+  Definition instRs :=
+    MethodSig ("pgm" -- "getRs")(): Data instBytes.
+
+  Definition f2dEnq := f2dEnq f2dElt.
+  Definition f2dDeq := f2dDeq f2dElt.
+
+  Definition w2dDeq := w2dDeq iaddrSize.
+
+  Definition RqFromProc := MemTypes.RqFromProc dataBytes (Bit addrSize).
+  Definition RsToProc := MemTypes.RsToProc dataBytes.
+
+  Definition memReq := memReq addrSize dataBytes.
+  Definition memRep := memRep dataBytes.
+
+  Variables (pcInit : ConstT (Pc iaddrSize)).
+
+  Definition fetcher := MODULE {
+    Register "pc" : Pc iaddrSize <- pcInit
+    with Register "pinit" : Bool <- Default
+    with Register "pinitRqOfs" : Bit iaddrSize <- Default
+    with Register "pinitRsOfs" : Bit iaddrSize <- Default
+    with Register "pinstRsOfs" : Bit iaddrSize <- Default
+    with Register "fEpoch" : Bool <- false
+    with Register "fStall" : Bool <- false
+
+    (** Phase 1: initialize the program [pinit == false] *)
+
+    with Rule "pgmInitRq" :=
+      Read pinit <- "pinit";
+      Assert !#pinit;
+      Read pinitRqOfs : Bit iaddrSize <- "pinitRqOfs";
+      Assert ((UniBit (Inv _) #pinitRqOfs) != $0);
+
+      Call memReq(STRUCT { "addr" ::= (_zeroExtend_ #pinitRqOfs) << $$(natToWord 2 2);
+                           "op" ::= $$false;
+                           "data" ::= $$Default });
+      Write "pinitRqOfs" <- #pinitRqOfs + $1;
+      Retv
+
+    with Rule "pgmInitRqEnd" :=
+      Read pinit <- "pinit";
+      Assert !#pinit;
+      Read pinitRqOfs : Bit iaddrSize <- "pinitRqOfs";
+      Assert ((UniBit (Inv _) #pinitRqOfs) == $0);
+      Call memReq(STRUCT { "addr" ::= (_zeroExtend_ #pinitRqOfs) << $$(natToWord 2 2);
+                           "op" ::= $$false;
+                           "data" ::= $$Default });
+      Retv
+        
+    with Rule "pgmInitRs" :=
+      Read pinit <- "pinit";
+      Assert !#pinit;
+      Read pinitRsOfs : Bit iaddrSize <- "pinitRsOfs";
+
+      Call ldData <- memRep();
+      LET ldVal <- #ldData!RsToProc@."data";
+      LET inst <- alignInst _ ldVal;
+      Call instRq(STRUCT { "write" ::= $$true;
+                           "addr" ::= #pinitRsOfs;
+                           "datain" ::= #inst });
+      Write "pinitRsOfs" <- #pinitRsOfs + $1;
+      Retv
+
+    with Rule "pgmInitAck" :=
+      Read pinit <- "pinit";
+      Assert !#pinit;
+      Read pinstRsOfs : Bit iaddrSize <- "pinstRsOfs";
+      Assert ((UniBit (Inv _) #pinstRsOfs) != $0);
+
+      Call instRs();
+      Write "pinstRsOfs" <- #pinstRsOfs + $1;
+      Retv
+        
+    with Rule "pgmInitAckEnd" :=
+      Read pinit <- "pinit";
+      Assert !#pinit;
+      Read pinstRsOfs : Bit iaddrSize <- "pinstRsOfs";
+      Assert ((UniBit (Inv _) #pinstRsOfs) == $0);
+
+      Call instRs();
+      Write "pinit" <- !#pinit;
+      Retv
+
+    (** Phase 2: execute the program [pinit == true] *)
+                                  
+    with Rule "modifyPc" :=
+      Read pinit <- "pinit";
+      Assert #pinit;
+      Read stall <- "fStall";
+      Assert !#stall;
+      Call correctPc <- w2dDeq();
+      Write "pc" <- #correctPc;
+      Read pEpoch <- "fEpoch";
+      Write "fEpoch" <- !#pEpoch;
+      Call f2dFlush();
+      Retv
+
+    with Rule "instFetchRq" :=
+      Read pinit <- "pinit";
+      Assert #pinit;
+      Read stall <- "fStall";
+      Assert !#stall;
+      Read pc : Pc iaddrSize <- "pc";
+      Call instRq(STRUCT { "write" ::= $$false;
+                           "addr" ::= _truncLsb_ #pc;
+                           "datain" ::= $$Default });
+      Write "fStall" <- $$true;
+      Retv
+
+    with Rule "instFetchRs" :=
+      Read pinit <- "pinit";
+      Assert #pinit;
+      Read stall <- "fStall";
+      Assert #stall;
+      Call inst <- instRs();
+      Read pc : Pc iaddrSize <- "pc";
+      Read epoch <- "fEpoch";
+      LET npc <- predictNextPc _ pc;
+      Call f2dEnq(f2dPack #inst #pc #npc #epoch);
+      Write "pc" <- #npc;
+      Write "fStall" <- $$false;
+      Retv
+  }.
+
+  Definition fetchICache := (fetcher ++ icache)%kami.
+
+End FetchICache.
+
+Hint Unfold fetcher icache fetchICache : ModuleDefs.
+Hint Unfold instRq instRs
+     f2dEnq f2dDeq w2dDeq RqFromProc RsToProc
+     memReq memRep: MethDefs.
+
+Section Facts.
+  Variables addrSize iaddrSize instBytes dataBytes rfIdx: nat.
+
+  Variables (fetch: AbsFetch instBytes dataBytes)
+            (predictNextPc:
+               forall ty, fullType ty (SyntaxKind (Pc iaddrSize)) -> (* pc *)
+                          Expr ty (SyntaxKind (Pc iaddrSize))).
+
+  Variable (d2eElt: Kind).
+  Variable (d2ePack:
+              forall ty,
+                Expr ty (SyntaxKind (Bit 2)) -> (* opTy *)
+                Expr ty (SyntaxKind (Bit rfIdx)) -> (* dst *)
+                Expr ty (SyntaxKind (Bit addrSize)) -> (* addr *)
+                Expr ty (SyntaxKind (Data dataBytes)) -> (* val1 *)
+                Expr ty (SyntaxKind (Data dataBytes)) -> (* val2 *)
+                Expr ty (SyntaxKind (Data instBytes)) -> (* rawInst *)
+                Expr ty (SyntaxKind (Pc iaddrSize)) -> (* curPc *)
+                Expr ty (SyntaxKind (Pc iaddrSize)) -> (* nextPc *)
+                Expr ty (SyntaxKind Bool) -> (* epoch *)
+                Expr ty (SyntaxKind d2eElt)).
+
+  Variable (f2dElt: Kind).
+  Variable (f2dPack:
+              forall ty,
+                Expr ty (SyntaxKind (Data instBytes)) -> (* rawInst *)
+                Expr ty (SyntaxKind (Pc iaddrSize)) -> (* curPc *)
+                Expr ty (SyntaxKind (Pc iaddrSize)) -> (* nextPc *)
+                Expr ty (SyntaxKind Bool) -> (* epoch *)
+                Expr ty (SyntaxKind f2dElt)).
+  Variables
+    (f2dRawInst: forall ty, fullType ty (SyntaxKind f2dElt) ->
+                            Expr ty (SyntaxKind (Data instBytes)))
+    (f2dCurPc: forall ty, fullType ty (SyntaxKind f2dElt) ->
+                          Expr ty (SyntaxKind (Pc iaddrSize)))
+    (f2dNextPc: forall ty, fullType ty (SyntaxKind f2dElt) ->
+                           Expr ty (SyntaxKind (Pc iaddrSize)))
+    (f2dEpoch: forall ty, fullType ty (SyntaxKind f2dElt) ->
+                          Expr ty (SyntaxKind Bool)).
+
+  Lemma fetcher_ModEquiv:
+    forall pcInit, ModPhoasWf (fetcher addrSize fetch predictNextPc f2dPack pcInit).
+  Proof. kequiv. Qed.
+  Hint Resolve fetcher_ModEquiv.
+
+  Lemma fetchICache_ModEquiv:
+    forall pcInit,
+      ModPhoasWf (fetchICache addrSize fetch predictNextPc f2dPack pcInit).
+  Proof.
+    kequiv.
+  Qed.
+
+End Facts.
+
+Hint Resolve fetcher_ModEquiv fetchICache_ModEquiv.
+
